%-----------------------------------------------------
% index key words
%-----------------------------------------------------
\index{matrix product}
\index{matrix power}

%-----------------------------------------------------
% name, leave blank
% title, if the exercise has a name i.e. Hilbert's matrix
% difficulty = n, where n is the number of stars
% origin = "\cite{ref}"
%-----------------------------------------------------
\begin{Exercise}[
name={},
title={}, 
difficulty=0,
origin={\cite{GH}}]
The following statement 
\[
(A+B)^2=A^2+2AB+B^2
\]
is false.  We investigate that claim here.
\Question Let $A=\begin{mat}5&3\\  -3&-2 \end{mat}$ and let $B=\begin{mat}-5&-5\\  -2&1 \end{mat}.$ Compute $A+B$
\Question Find $(A+B)^2$ by using the previous part.
\Question Compute $A^2+2AB+B^2$.
\Question Are the results from the two previous parts equal?
\Question Carefully expand the expression $(A+B)^2 = (A+B)(A+B)$ and show why this is not equal to $A^2+2AB+B^2$.
\end{Exercise}

\begin{Answer}
\Question $\begin{mat}0&-2\\-5&-1 \end{mat}$
\Question $\begin{mat}10&2\\  5&11 \end{mat}$
\Question $\begin{mat}-11&-15\\  37&32\end{mat}$
\Question No.
\Question $(A+B)=AA+AB+BA+BB=A^2+AB+BA+B^2$
\end{Answer}
